\begin{exercise}
      {ID-7683fce5404f0fb20fa052e75129a1640f25cf58}
      {Äquivalenzumformungen: Jede Variable}
  \ifproblem\problem\par
    % <PROBLEM>
    Löse folgende Gleichungen nach jeder jeweils vorkommenden Variable auf:
    \begin{equation*}
      \text{a)}\;\;
      2a=\frac{b}{1+cd}
      \quad
      \quad
      \text{b)}\;\;
      \frac{a}{b}+a=1-c
      \quad
      \quad
      \text{c)}\;\;
      \frac{a+b}{a-b}=\frac{c-d}{c+d}
      \quad
      \quad
      \text{d)}\;\;
      \frac{ab}{a-b}=\frac{c-d}{cd}
    \end{equation*}
    % </PROBLEM>
  \fi
  %\ifoutline\outline\par
    % <OUTLINE>
    % </OUTLINE>
  %\fi
  \ifoutcome\outcome\par
    % <OUTCOME>
    \begingroup
      % Hilfsmakros
      \newcommand{\vstrut}{\vphantom{\left(\frac{h}{q}\right)}}%
      \newcommand{\equi}{\Leftrightarrow&\vstrut\quad}%
      \newcommand{\calc}[1]
      {%
        \ifthenelse{\equal{#1}{}}%
        {%
          \quad&%
        }%
        {%
          \quad&|\,#1%
        }%
      }%
      \newcommand{\ccalc}[2]%
      {%
        \calc{#1}\quad|\,#2%
      }%
      % ------------
      Teilaufgabe a)
      % ------------
      \begin{alignat*}{3}
        \relax&\vstrut\quad
        &
        2a&=\frac{b}{1+cd}
        &
        \calc{:2}
        \\
        \equi
        &
        a&=\frac{b}{2\cdot(1+cd)}
        &
        \quad&\relax
        \\[2ex]
        \relax&\vstrut\quad
        &
        2a&=\frac{b}{1+cd}
        &
        \calc{\cdot(1+cd)}
        \\
        \equi
        &
        2a\cdot(1+cd)&=b
        &
        \calc{:(2a)}
        \\
        \equi
        &
        1+cd&=\frac{b}{2a}
        &
        \calc{-1}
        \\
        \equi
        &
        cd&=\frac{b}{2a}-1
        &
        \calc{:d}
        \\
        \equi
        &
        c&=\frac{b}{2ad}-\frac{1}{d}
        &
        \calc{}
        \\
        \equi
        &
        c&=\frac{b-2a}{2ad}
        &
        \ccalc{\cdot d}{:c}
        \\
        \equi
        &
        d&=\frac{b-2a}{2ac}
        &
        \calc{}
      \end{alignat*}
      % ------------
      Teilaufgabe b)
      % ------------
      \begin{alignat*}{3}
        \relax&\vstrut\quad
        &
        \frac{a}{b}+a&=1-c
        &
        \calc{\cdot b}
        \\
        \equi
        &
        a+ab&=(1-c)\cdot b
        &
        \calc{}
        \\
        \equi
        &
        a\cdot(1+b)&=(1-c)\cdot b
        &
        \calc{:(1+b)}
        \\
        \equi
        &
        a&=\frac{1-c}{1+b}\cdot b
        &
        \calc{}
        \\
        \equi
        &
        a&=\frac{b-bc}{1+b}
        &
        \calc{}
      \end{alignat*}
      \begin{alignat*}{3}
        \relax&\vstrut\quad
        &
        \frac{a}{b}+a&=1-c
        &
        \calc{-a}
        \\
        \equi
        &
        \frac{a}{b}&=1-c-a
        &
        \calc{\cdot b}
        \\
        \equi
        &
        a&=(1-c-a)\cdot b
        &
        \calc{:(1-c-a)}
        \\
        \equi
        &
        \frac{a}{1-a-c}&=b
        &
        \calc{}
      \end{alignat*}
      \begin{alignat*}{3}
        \relax&\vstrut\quad
        &
        \frac{a}{b}+a&=1-c
        &
        \calc{-1}
        \\
        \equi
        &
        \frac{a}{b}+a-1&=-c
        &
        \calc{\cdot(-1)}
        \\
        \equi
        &
        1-a-\frac{a}{b}&=c
        &
        \calc{}
        \\
        \equi
        &
        \frac{b-ab-a}{b}&=c
        &
        \calc{}
      \end{alignat*}
      % ------------
      Teilaufgabe c)
      % ------------
      \begin{alignat*}{3}
        \relax&\vstrut\quad
        &
        \frac{a+b}{a-b}&=\frac{c-d}{c+d}
        &
        \ccalc{\cdot(a-b)}{\cdot(c+d)}
        \\
        \equi
        &
        (a+b)(c+d)&=(c-d)(a-b)
        &
        \calc{}
        \\
        \equi
        &
        a\cdot(c+d)+b\cdot(c+d)&=a\cdot(c-d)-b\cdot(c-d)
        &
        \ccalc{-b\cdot(c+d)}{-a\cdot(c-d)}
        \\
        \equi
        &
        a\cdot(c+d)-a\cdot(c-d)&=-b\cdot(c-d)-b\cdot(c+d)
        &
        \calc{}
        \\
        \equi
        &
        a\cdot((c+d)-(c-d))&=b\cdot(-(c-d)-(c+d))
        &
        \calc{}
        \\
        \equi
        &
        2ad&=-2bc
        &
        \calc{:2}
        \\
        \equi
        &
        ad&=-bc
        &
        \calc{}
      \end{alignat*}
      Daraus folgt unmittelbar:
      \begin{equation*}
        a=-\frac{bc}{d}
        \qquad
        \qquad
        d=-\frac{bc}{a}
        \qquad
        \qquad
        b=-\frac{ad}{c}
        \qquad
        \qquad
        c=-\frac{ad}{b}
      \end{equation*}
      % ------------
      Teilaufgabe d)
      % ------------
      \begin{alignat*}{3}
        \relax&\vstrut\quad
        &
        \frac{ab}{a-b}&=\frac{c-d}{cd}
        &
        \ccalc{\cdot(a-b)}{\cdot cd}
        \\
        \equi
        &
        abcd&=(a-b)(c-d)
        &
        \calc{}
        \\
        \equi
        &
        abcd&=a\cdot(c-d)-b\cdot(c-d)
        &
        \calc{-a\cdot(c-d)}
        \\
        \equi
        &
        abcd-a\cdot(c-d)&=-b\cdot(c-d)
        &
        \calc{}
        \\
        \equi
        &
        a\cdot(bcd-c+d)&=-b\cdot(c-d)
        &
        \calc{:(bcd-c+d)}
        \\
        \equi
        &
        a&=\frac{-b\cdot(c-d)}{bcd-c+d}
        &
        \calc{}
        \\
        \equi
        &
        a&=\frac{b\cdot(d-c)}{bcd-c+d}
        &
        \calc{}
      \end{alignat*}
      \begin{alignat*}{3}
        \relax&\vstrut\quad
        &
        \frac{ab}{a-b}&=\frac{c-d}{cd}
        &
        \ccalc{\cdot(a-b)}{\cdot cd}
        \\
        \equi
        &
        abcd&=(a-b)(c-d)
        &
        \calc{}
        \\
        \equi
        &
        abcd&=a\cdot(c-d)-b\cdot(c-d)
        &
        \calc{+b\cdot(c-d)}
        \\
        \equi
        &
        abcd+b\cdot(c-d)&=a\cdot(c-d)
        &
        \calc{}
        \\
        \equi
        &
        b\cdot(acd+c-d)&=a\cdot(c-d)
        &
        \calc{:(acd+c-d)}
        \\
        \equi
        &
        b&=\frac{a\cdot(c-d)}{acd+c-d}
        &
        \calc{}
      \end{alignat*}
      \begin{alignat*}{3}
        \relax&\vstrut\quad
        &
        \frac{ab}{a-b}&=\frac{c-d}{cd}
        &
        \ccalc{\cdot(a-b)}{\cdot cd}
        \\
        \equi
        &
        abcd&=(a-b)(c-d)
        &
        \calc{}
        \\
        \equi
        &
        abcd&=c\cdot(a-b)-d\cdot(a-b)
        &
        \calc{-c\cdot(a-b)}
        \\
        \equi
        &
        abcd-c\cdot(a-b)&=-d\cdot(a-b)
        &
        \calc{}
        \\
        \equi
        &
        c\cdot(abd-a+b)&=-d\cdot(a-b)
        &
        \calc{:(abd-a+b)}
        \\
        \equi
        &
        c&=\frac{-d\cdot(a-b)}{abd-a+b}
        &
        \calc{}
        \\
        \equi
        &
        c&=\frac{d\cdot(b-a)}{abd-a+b}
        &
        \calc{}
      \end{alignat*}
      \begin{alignat*}{3}
        \relax&\vstrut\quad
        &
        \frac{ab}{a-b}&=\frac{c-d}{cd}
        &
        \ccalc{\cdot(a-b)}{\cdot cd}
        \\
        \equi
        &
        abcd&=(a-b)(c-d)
        &
        \calc{}
        \\
        \equi
        &
        abcd&=c\cdot(a-b)-d\cdot(a-b)
        &
        \calc{+d\cdot(a-b)}
        \\
        \equi
        &
        abcd+d\cdot(a-b)&=c\cdot(a-b)
        &
        \calc{}
        \\
        \equi
        &
        d\cdot(abc+a-b)&=c\cdot(a-b)
        &
        \calc{:(abc+a-b)}
        \\
        \equi
        &
        d&=\frac{c\cdot(a-b)}{abc+a-b}
        &
        \calc{}
      \end{alignat*}
    \endgroup
    % </OUTCOME>
  \fi
\end{exercise}
